\chapter{Appdx A:Dynamic Equation for Passive Walking}

\section*{Knee Free Phase}

\[
M(q)\ddot{q}+C(q,\dot{q})\dot{q}+N=\tau\]


\[
M(q)=\left[\begin{array}{ccc}
M_{11} & M_{12} & M_{13}\\
M_{12} & M_{22} & M_{23}\\
M_{13} & M_{23} & M_{33}\end{array}\right]
\]

\[
M_{11}=m_{s}^{st}a_{1}^{2}+m_{t}^{st}(l_{s}+a_{2})^{2}+(m_{h}+m_{t}^{sw}+m_{s}^{sw})L^{2}\]


\[
M_{12}=-(m_{t}^{sw}b_{2}+m_{s}^{sw}l_{t})Lcos(q_{2}-q_{1})\]


\[
M_{13}=-m_{s}^{sw}b_{1}cos(q_{3}-q_{1})\]


\[
M_{22}=m_{t}^{sw}b_{2}^{2}+m_{s}^{sw}l_{t}^{2}\]
\[
M_{23}=m_{s}^{sw}l_{t}b_{1}cos(q_{3}-q_{2})\]


\[
M_{33}=m_{s}^{sw}b_{1}^{2}\]


\[
C(q,\dot{q})=\left[\begin{array}{ccc}
0 & C_{12}\dot{q_{2}} & C_{13}\dot{q}_{3}\\
-C_{12}\dot{q}_{1} & 0 & C_{23}\dot{q}_{3}\\
-C_{13}\dot{q_{1}} & -C_{23}\dot{q}_{2} & 0\end{array}\right]\]


\[
C_{12}=-(m_{t}^{sw}b_{2}+m_{s}^{sw}l_{t})Lsin(q_{1}-q_{2})\]


\[
C_{13}=-m_{s}^{sw}b_{1}Lsin(q_{1}-q_{3})\]


\[
C_{23}=m_{s}^{sw}l_{t}b_{1}sin(q_{3}-q_{2})\]



\[
N=\left[\begin{array}{c}
-(m_{s}^{st}a_{1}+m_{t}^{st}(l_{s}+a_{2})+(m_{h}+m_{s}^{sw}+m_{t}^{sw})L)g\mathbf{\mathrm{sin}}(q_{1})\\
(m_{t}^{sw}b_{2}+m_{s}^{sw}l_{t})gsin(q_{2})\\
m_{s}^{sw}b_{1}gsin(q_{3})\end{array}\right]\]


\section*{Knee Strike}

\[
Q^{+}\left[\begin{array}{c}
\dot{q}_{1}\\
\dot{q}_{2}\end{array}\right]^{+}=Q^{-}\left[\begin{array}{c}
\dot{q}_{1}\\
\dot{q}_{2}\\
\dot{q}_{3}\end{array}\right]^{-}\]


\[
q_{3}^{+}=q_{2}^{+}\]


\[
Q^{-}=\left[\begin{array}{ccc}
Q_{11}^{-} & Q_{12}^{-} & Q_{13}^{-}\\
Q_{21}^{-} & Q_{22}^{-} & Q_{23}^{-}\end{array}\right]\]


\[
Q^{+}=\left[\begin{array}{cc}
Q_{11}^{+} & Q_{12}^{+}\\
Q_{21}^{+} & Q_{22}^{+}\end{array}\right]\]


\[
Q_{11}^{-}=-(m_{s}^{sw}l_{t}+m_{t}^{sw}b_{2})Lcos(q_{1}-q_{2})-m_{s}^{sw}b_{1}cos(q_{1}-q_{3})+(m_{t}^{sw}+m_{s}^{sw}+m_{h})L^{2}+m_{s}^{st}a_{1}^{2}+m_{t}^{st}(l_{s}+a_{2})^{2}\]


\[
Q_{12}^{-}=-(m_{s}^{sw}l_{s}+m_{t}^{sw})Lcos(q_{1}-q_{2})+m_{s}^{sw}b_{1}l_{t}cos(q_{2}-q_{3})+m_{t}^{sw}b_{2}^{2}+m_{s}^{sw}l_{t}^{2}\]


\[
Q_{13}^{-}=-m_{s}^{sw}b_{1}Lcos(q_{1}-q_{3})+m_{s}^{sw}b_{1}l_{t}cos(q_{2}-q_{3})+m_{s}^{sw}b_{1}b_{2}\]


\[
Q_{21}^{-}=-(m_{s}^{sw}l_{t}+m_{t}^{sw}b_{2})Lcos(q_{1}-q_{2})-m_{s}^{sw}b_{1}Lcos(q_{1}-q_{3})\]


\[
Q_{22}^{-}=m_{s}^{sw}b_{1}l_{t}cos(q_{2}-q_{3})+m_{s}^{sw}l_{t}^{2}+m_{t}^{sw}b_{2}^{2}\]
\[
Q_{23}^{-}=m_{s}^{sw}b_{1}l_{t}cos(q_{2}-q_{3})+m_{s}^{sw}b_{1}^{2}\]


\[
Q_{11}^{+}=Q_{21}^{+}+m_{t}^{st}(l_{s}+a_{2})^{2}+(m_{h}+m_{t}^{sw}+m_{s}^{sw})L^{2}+m_{s}^{st}a_{1}^{2}\]


\[
Q_{12}^{+}=Q_{21}^{+}+m_{s}^{sw}(l_{t}+b_{1})^{2}+m_{t}^{sw}b_{2}^{2}\]


\[
Q_{21}^{+}=-(m_{s}^{sw}(b_{1}+l_{t})+m_{t}^{sw}b_{2})Lcos(q_{1}-q_{2})\]


\[
Q_{22}^{+}=m_{s}^{sw}(b_{1}+l_{t})^{2}+m_{t}^{sw}b_{2}^{2}\]



\section*{Knee Lock Phase}


\[
M(q)\ddot{q}+C(q,\dot{q})\dot{q}+N=\tau\]


\[M(q)=\left[\begin{array}{cc}
M_{11} & M_{12}\\
M_{12} & M_{22}\end{array}\right]
\]

\[
M_{11}=m_{s}^{st}a_{1}^{2}+m_{t}^{st}(l_{s}+a_{2})^{2}+(m_{h}+m_{t}^{sw}+m_{s}^{sw})L^{2}\]


\[
M_{12}=-(m_{t}^{sw}b_{2}+m_{s}(l_{t}+b_{1}))Lcos(q_{2}-q_{1})\]


\[
C(q,\dot{q})=\left[\begin{array}{cc}
0 & C_{12}\dot{q}_{2}\\
-C_{12}\dot{q}_{1} & 0\end{array}\right]
\]

\[
C_{12}=(m_{t}^{sw}b_{2}+m_{s}(l_{t}+b_{1}))Lsin(q_{1}-q_{2})
\]

\[
N=\left[\begin{array}{c}
-(m_{s}^{st}a_{1}+m_{t}^{st}(l_{s}+a_{2})+(m_{h}+m_{s}^{sw}+m_{t}^{sw})L)g\mathbf{\mathrm{sin}}(q_{1})\\
(m_{t}^{sw}b_{2}+m_{s}^{sw}(l_{t}+b_{1}))gsin(q_{2})\end{array}\right]
\]

\section*{Heel Strike Phase}

\[
Q^{+}\dot{q}^{+}=Q^{-}\dot{q}^{-}\]



\[
q^{+}=\left[\begin{array}{cc}
0 & 1\\
1 & 0\\
1 & 0\end{array}\right]q^{-}\]




\[
\dot{q}_{3}^{+}=\dot{q}_{2}^{+}\]


\[
Q^{-}=\left[\begin{array}{cc}
Q_{11}^{-} & Q_{22}^{-}\\
Q_{21}^{-} & 0\end{array}\right]\]


\[
Q_{11}^{-}=Q_{21}^{-}+(m_{h}L+m_{t}^{st}(a_{2}+l_{s})+m_{s}^{st}a_{1}+m_{t}^{sw}(a_{2}+l_{s})+m_{s}a_{1})Lcos(q_{1}-q_{2})\]


\[
Q_{12}^{-}=-m_{s}^{sw}a_{1}(l_{t}+b_{1})-m_{t}^{sw}b_{2}(l_{s}+a_{2})\]


\[
Q_{21}^{-}=-m_{s}^{st}a_{1}(l_{t}+b_{1})-m_{t}^{st}b_{2}(l_{s}+a_{2})\]



\[
Q_{11}^{+}=Q_{21}^{+}+(m_{s}^{st}+m_{t}^{st}+m_{h})L^{2}+m_{s}^{sw}a_{1}^{2}+m_{t}^{sw}(a_{2}+l_{s})^{2}\]


\[
Q_{12}^{+}=Q_{21}^{+}+(m_{s}^{st}+m_{t}^{st}+m_{h})L^{2}+m_{s}^{sw}a_{1}^{2}+m_{t}^{sw}(a_{2}+l_{s})^{2}\]


\[
Q_{21}^{+}=-(m_{s}^{st}(b_{1}+l_{t})+m_{t}^{st}b_{2})Lcos(q_{1}-q_{2})\]


\[
Q_{22}^{+}=m_{s}^{st}(l_{t}+b_{1})^{2}+m_{t}^{st}b_{2}^{2}\]






% ------------------------------------------------------------------------

%%% Local Variables: 
%%% mode: latex
%%% TeX-master: "../thesis"
%%% End: 
